LogRel/SN/Defs.lean
@@ -1,8 +1,0 @@
-
-
-import LogRel.SmallStep
-import LogRel.Typing
-def termination (e : Expr) :=
-  ∃ v, value v ∧ stepn e v
-
-theorem strong_normalization : ∀ Γ e τ, typing Γ e τ → termination e := by admit
