LogRel/STLC/SN.lean
@@ -1,0 +1,55 @@
+
+
+import LogRel.STLC.SmallStep
+import LogRel.STLC.Typing
+@[simp]
+def normalizable (e : Expr) :=
+  ∃ v, value v ∧ stepn e v
+
+@[simp]
+def SN : Expr → Ty → Prop
+  | e, .unit => normalizable e
+  | f, .arrow τ𝕒 τ𝕓 => normalizable f ∧ ∀ arg, SN arg τ𝕒 → SN (.app f arg) τ𝕓
+
+theorem SN_impl_normalizable : ∀ e τ, SN e τ → normalizable e :=
+  by
+  intros e τ HSN
+  induction τ
+  case unit => apply HSN
+  case arrow => apply HSN.left
+
+theorem SN_reduction : ∀ e₀ e₁ τ, typing [] e₀ τ → step e₀ e₁ → (SN e₀ τ ↔ SN e₁ τ) := by
+  intros e₀ e₁ τ Hτ Hstep
+  cases Hstep
+  case step𝕄 HM Hhead =>
+    induction HM generalizing τ
+    case hole => admit
+    case cons𝔹 HB HM IH =>
+      cases HB
+      case appl => admit
+      case appr => admit
+
+example : ∀ e τ, typing [] e τ → SN e τ := by
+  generalize HEqΓ : [] = Γ
+  intros e τ Hτ
+  induction Hτ
+  case fvar Hbinds =>
+    rw [← HEqΓ] at Hbinds
+    nomatch Hbinds
+  case lam e _ _ _ IH =>
+    constructor
+    . exists .lam e
+      constructor
+      . apply value.lam
+      . apply stepn.refl
+    . admit
+  case app IHf IHarg =>
+    apply (IHf HEqΓ).right
+    apply (IHarg HEqΓ)
+  case unit =>
+    exists .unit
+    constructor
+    . apply value.unit
+    . apply stepn.refl
+
+theorem strong_normalization : ∀ e τ, typing [] e τ → normalizable e := by admit
